examples/new_stack/NewStack23Bproof.v
@@ -33,6 +33,303 @@ Section SIMMODSEM.
 
   Let W: Type := ((Σ * Any.t)) * ((Σ * Any.t)).
 
+  Notation sim stk_res0 stk_mgr0 :=
+    (∀ h,
+        (∃ P stk, <<SRC: (stk_res0: URA.car (t:=_stkRA)) h = Some (Ag.ag P)>> ∧
+                         <<TGT: (stk_mgr0: gmap mblock (list Z)) !! h = Some stk>> ∧ <<PR: Forall P stk>>) ∨
+        (<<SRC: (stk_res0: URA.car (t:=_stkRA)) h = None>> ∧
+                <<TGT: (stk_mgr0: gmap mblock (list Z)) !! h = None>>)
+    )
+  .
+(*   match (stk_res0: URA.car (t:=_stkRA)) h with *)
+(*   | Some P => ∃ stk, <<TGT: (stk_mgr0: gmap mblock (list Z)) !! h = Some stk>> ∧ <<PR: Forall P stk>> *)
+(*   | None => <<TGT: (stk_mgr0: gmap mblock (list Z)) !! h = None>> *)
+(*   end) *)
+
+  Let wf: W -> Prop :=
+    @mk_wf _ unit
+           (fun _ _ _stk_mgr0 =>
+              (∃ stk_mgr0 (stk_res0: URA.car (t:=_stkRA)),
+                  (⌜(<<PHYS: _stk_mgr0 = stk_mgr0↑>>) /\ (<<SIM: sim stk_res0 stk_mgr0>>)⌝)
+                  ∧ (OwnM ((Auth.black stk_res0): URA.car (t:=stkRA)))
+              )%I)
+           (fun _ _ _ => ⌜True⌝%I)
+  .
+
+  Section AUX.
+    Context {K: Type} `{M: URA.t}.
+    Let RA := URA.pointwise K M.
+
+    Lemma pw_extends (f0 f1: K -> M) (EXT: @URA.extends RA f0 f1): <<EXT: forall k, URA.extends (f0 k) (f1 k)>>.
+    Proof. ii. r in EXT. des. subst. ur. ss. eexists; et. Qed.
+
+    Lemma pw_wf: forall (f: K -> M) (WF: URA.wf (f: @URA.car RA)), <<WF: forall k, URA.wf (f k)>>.
+    Proof. ii; ss. rewrite URA.unfold_wf in WF. ss. Qed.
+
+    Lemma pw_add_disj_wf
+          (f g: K -> M)
+          (WF0: URA.wf (f: @URA.car RA))
+          (WF1: URA.wf (g: @URA.car RA))
+          (DISJ: forall k, <<DISJ: f k = ε \/ g k = ε>>)
+      :
+        <<WF: URA.wf ((f: RA) ⋅ g)>>
+    .
+    Proof.
+      ii; ss. ur. i. ur in WF0. ur in WF1. spc DISJ. des; rewrite DISJ.
+      - rewrite URA.unit_idl; et.
+      - rewrite URA.unit_id; et.
+    Qed.
+
+    Lemma pw_insert_wf: forall `{EqDecision K} (f: K -> M) k v (WF: URA.wf (f: @URA.car RA)) (WFV: URA.wf v),
+        <<WF: URA.wf (<[k:=v]> f: @URA.car RA)>>.
+    Proof.
+      i. unfold insert, fn_insert. ur. ii. des_ifs. ur in WF. eapply WF.
+    Qed.
+
+  End AUX.
+
+  Variable global_stb: list (string * fspec).
+  Hypothesis STBINCL: stb_incl (DebugStb ++ StackStb) global_stb.
+
+  Lemma _is_stack_wf
+        h stk
+    :
+      <<WF: URA.wf (_is_stack h stk)>>
+  .
+  Proof. ur. ur. i. unfold _is_stack. des_ifs; ur; ss. i; clarify. Qed.
+
+  Lemma sim_update
+        stk_res0
+        stk_mgr0
+        (SIM: sim stk_res0 stk_mgr0)
+        (h: mblock) P (stk: (list Z))
+        (PR: Forall P stk)
+    :
+      <<SIM: sim (<[h:=Some (Ag.ag P)]>stk_res0) (<[h:=stk]> stk_mgr0)>>
+  .
+  Proof.
+    ii.
+    destruct (dec h h0).
+    - subst. rewrite ! lookup_insert. unfold insert, fn_insert. des_ifs. ss. left. esplits; et.
+    - rewrite lookup_insert_ne; ss. unfold insert, fn_insert. des_ifs.
+  Qed.
+
+  Lemma add_disj_insert
+        (stk_res0: _stkRA) h P
+        (DISJ: stk_res0 h = ε)
+    :
+        (stk_res0 ⋅ _is_stack h P) = <[h:=Some (Ag.ag P)]>stk_res0
+  .
+  Proof.
+    unfold insert, fn_insert. extensionality b. ur. unfold _is_stack. des_ifs.
+    - rewrite DISJ. rewrite URA.unit_idl. ss.
+    - rewrite URA.unit_id. ss.
+  Qed.
+
+  Theorem sim_modsem: ModSemPair.sim (NewStack3B.StackSem global_stb) (NewStack2.StackSem).
+  Proof.
+    econstructor 1 with (wf:=wf); ss; et; swap 2 3.
+    { econs; ss.
+      - eapply to_semantic; cycle 1. { admit "ez - wf". } iIntros "H". iExists _, _. iSplit; ss; et.
+        iSplit; ss; et.
+      - eapply to_semantic; cycle 1. { eapply URA.wf_unit. } iIntros "H". iPureIntro. ss.
+    }
+    econs; ss.
+    { unfold NewStack2.new_body, cfun. init. harg. fold wf. mDesAll. des; clarify.
+      apply Any.upcast_inj in PURE0. des; clarify. steps. rewrite Any.upcast_downcast in *. clarify. steps.
+      astart 0. astop. steps. rewrite Any.upcast_downcast in *. clarify.
+      rename g into stk_mgr0. rename x0 into h. rename a1 into stk_res0. rename x into P. des_u.
+      force_l. exists (Vptr h 0). steps.
+      mOwnWf "A".
+      (* assert(WF1: forall k, stk_res0 k <> Excl.boom). *)
+      (* { eapply Auth.black_wf in WF0. eapply pw_wf in WF0. des. ii. specialize (WF0 k). *)
+      (*   destruct (stk_res0 k); ss. ur in WF0; ss. } *)
+
+      hret _; ss.
+      { iPoseProof (OwnM_Upd with "A") as "A".
+        { eapply Auth.auth_alloc2. instantiate (1:=(_is_stack h P)).
+          rewrite add_disj_insert; ss.
+          { eapply (@pw_insert_wf); et.
+            { eapply Auth.black_wf; et. }
+            { ur; ss. eapply Ag.wf. }
+          }
+          specialize (SIM h). des; clarify.
+        }
+        iMod "A". iDestruct "A" as "[A B]". iModIntro. iSplitL "A"; et.
+        iExists _, _. iSplit; ss; et. iSplit; ss; et. iPureIntro. ii.
+        assert(B: stk_res0 h = None).
+        { destruct (stk_res0 h) eqn:T; ss. specialize (SIM h). des; clarify. }
+        rewrite add_disj_insert; ss. eapply sim_update; et.
+      }
+    }
+    econs; ss.
+    { unfold NewStack2.pop_body, cfun. init. harg. fold wf. des_ifs_safe. mDesAll. des; clarify.
+      steps. rewrite Any.upcast_downcast in *. clarify. steps.
+      astart 0. astop. steps. apply Any.upcast_inj in PURE0. des; clarify.
+      rename a0 into stk_mgr0. rename n into h. rename a1 into stk_res0.
+      mCombine "A1" "A".
+      mOwnWf "A1".
+      (* assert(A: forall k, URA.wf ((stk_res0 k): URA.car (t:=Excl.t _))). *)
+      (* { eapply URA.wf_mon in WF0. *)
+      (*   eapply Auth.black_wf in WF0. eapply pw_wf in WF0. des. ii. specialize (WF0 k). ss. } *)
+      assert(B: stk_res0 h = Some (Ag.ag P)).
+      { dup WF0.
+        eapply Auth.auth_included in WF0. des. unfold _is_stack in WF0. eapply pw_extends in WF0. des.
+        spc WF0. des_ifs. TTTTTTTTTTTTTTTTTT ss. eapply Excl.extends in WF0; ss. }
+      assert(C:=B). eapply SIM in C. rewrite C. steps.
+      destruct stk0 as [|x stk1].
+      - steps. hret _; ss. iDestruct "A1" as "[A B]". iModIntro. iFrame. iSplit; ss; et.
+      - steps.
+        destruct (alist_find "debug" (DebugStb ++ StackStb)) eqn:U; cycle 1.
+        { exfalso. stb_tac. ss. }
+        dup U. revert U. stb_tac. clarify. i.
+        apply STBINCL in U. rewrite U. steps. rewrite Any.upcast_downcast. steps.
+
+        set (stk_res1:=<[h:=Excl.just stk1]>stk_res0).
+        assert(WF1: URA.wf (stk_res1: URA.car (t:=_stkRA))).
+        { subst stk_res1. eapply (@pw_insert_wf); et.
+          { eapply URA.wf_mon in WF0. eapply Auth.black_wf in WF0. ss. }
+          ur; ss.
+        }
+
+        mAssert _ with "A1".
+        { iApply (OwnM_Upd with "A1").
+          eapply Auth.auth_update with (a':=stk_res1) (b':=_is_stack h (stk1)).
+          bar. ii. ss. des. clarify. esplits; et.
+          assert(D: ctx0 h = Excl.unit).
+          { clear - B. repeat ur in B. unfold _is_stack in *. des_ifs. }
+          extensionality h0. subst stk_res1. unfold insert, fn_insert. des_ifs. 
+          - ur. rewrite D. unfold _is_stack. ur. des_ifs.
+          - unfold _is_stack. ur. des_ifs.
+        }
+        mUpd "A". mDesOwn "A".
+
+        assert(SIM0: sim (<[h:=Excl.just stk1]> stk_res0) (<[h:=stk1]> stk_mgr0)).
+        { eapply sim_update; et. }
+
+        hcall _ _ _ with "A"; ss; et.
+        { iModIntro. iSplit; ss. iExists _, stk_res1. iSplit; ss; et. }
+        { ss. admit "this will be removed in open setting; it should be ord_top". }
+        steps. mDesAll. subst. des; clarify.
+
+        hret _; ss.
+        iModIntro. iFrame. iSplit; ss. iExists _, _; ss; et.
+    }
+    econs; ss.
+    { unfold NewStack2.push_body, cfun. init. harg. fold wf. des_ifs_safe. mDesAll. des; clarify.
+      steps. rewrite Any.upcast_downcast in *. clarify. steps.
+      astart 0. astop. steps. rewrite Any.upcast_downcast in *. clarify.
+      rename g into stk_mgr0. rename n into h. rename a1 into stk_res0. rename l into stk0. rename z into x.
+      mCombine "A1" "A".
+      mOwnWf "A1".
+      assert(A: forall k, URA.wf ((stk_res0 k): URA.car (t:=Excl.t _))).
+      { eapply URA.wf_mon in WF0.
+        eapply Auth.black_wf in WF0. eapply pw_wf in WF0. des. ii. specialize (WF0 k). ss. }
+      assert(B: stk_res0 h = Some stk0).
+      { dup WF0.
+        eapply Auth.auth_included in WF0. des. unfold _is_stack in WF0. eapply pw_extends in WF0. des.
+        spc WF0. des_ifs. ss. eapply Excl.extends in WF0; ss. }
+      assert(C:=B). eapply SIM in C. rewrite C. steps.
+
+      destruct (alist_find "debug" (DebugStb ++ StackStb)) eqn:U; cycle 1.
+      { exfalso. stb_tac. ss. }
+      dup U. revert U. stb_tac. clarify. i.
+      apply STBINCL in U. rewrite U. steps. rewrite Any.upcast_downcast. steps.
+
+      set (stk_res1:=<[h:=Excl.just (x::stk0)]>stk_res0).
+      assert(WF1: URA.wf (stk_res1: URA.car (t:=_stkRA))).
+      { subst stk_res1. eapply (@pw_insert_wf); et.
+        { eapply URA.wf_mon in WF0. eapply Auth.black_wf in WF0. ss. }
+        ur; ss.
+      }
+
+      mAssert _ with "A1".
+      { iApply (OwnM_Upd with "A1").
+        eapply Auth.auth_update with (a':=stk_res1) (b':=_is_stack h (x::stk0)).
+        bar. ii. ss. des. clarify. esplits; et.
+        assert(D: ctx0 h = Excl.unit).
+        { clear - B. repeat ur in B. unfold _is_stack in *. des_ifs. }
+        extensionality h0. subst stk_res1. unfold insert, fn_insert. des_ifs. 
+        - ur. rewrite D. unfold _is_stack. ur. des_ifs.
+        - unfold _is_stack. ur. des_ifs.
+      }
+      mUpd "A". mDesOwn "A".
+
+      assert(SIM0: ∀ h0 stk, <[h:=Excl.just (x::stk0)]> stk_res0 h0 = Excl.just stk ↔
+                             <[h:=(x::stk0)]> stk_mgr0 !! h0 = Some stk).
+      { eapply sim_update; et. }
+
+      hcall _ _ _ with "A"; ss; et.
+      { iModIntro. iSplit; ss. iExists _, stk_res1. iSplit; ss; et. }
+      { ss. admit "ditto". }
+      steps. mDesAll. subst. des; clarify.
+
+      hret _; ss.
+      iModIntro. iFrame. iSplit; ss. iExists _, _; ss; et.
+    }
+  Unshelve.
+    all: ss.
+  Qed.
+
+End SIMMODSEM.
+
+
+
+Section SIMMOD.
+
+  Context `{Σ: GRA.t}.
+  Context `{@GRA.inG stkRA Σ}.
+
+  Variable global_stb: Sk.t -> list (string * fspec).
+  Hypothesis STBINCL: forall sk, stb_incl (DebugStb ++ StackStb) (global_stb sk).
+
+  Theorem correct: ModPair.sim (NewStack3A.Stack global_stb) (NewStack2.Stack).
+  Proof.
+    econs; ss.
+    { ii. eapply adequacy_lift. eapply sim_modsem; ss. }
+    ii; ss. repeat (Psimpl; econs; ss).
+  Qed.
+
+End SIMMOD.
+
+
+
+
+Require Import NewStackHeader NewStack2 NewStack3B HoareDef SimModSem.
+Require Import Coqlib.
+Require Import Universe.
+Require Import Skeleton.
+Require Import PCM.
+Require Import ModSem Behavior.
+Require Import Relation_Definitions.
+
+(*** TODO: export these in Coqlib or Universe ***)
+Require Import Relation_Operators.
+Require Import RelationPairs.
+From ITree Require Import
+     Events.MapDefault.
+From ExtLib Require Import
+     Core.RelDec
+     Structures.Maps
+     Data.Map.FMapAList.
+Require Import TODOYJ.
+Require Import HTactics Logic IPM.
+Require Import OpenDef STB.
+Require Import TODO.
+
+Set Implicit Arguments.
+
+Local Open Scope nat_scope.
+
+
+
+Section SIMMODSEM.
+
+  Context `{Σ: GRA.t}.
+  Context `{@GRA.inG stkRA Σ}.
+
+  Let W: Type := ((Σ * Any.t)) * ((Σ * Any.t)).
+
   Let wf: W -> Prop :=
     @mk_wf _ unit
            (fun _ _ _stk_mgr0 =>
